More refactor

CpcMini/Rules/Common.lean
@@ -29,6 +29,10 @@ def eo_has_smt_translation (t : Term) : Prop :=
 def eo_has_bool_type (t : Term) : Prop :=
   __smtx_typeof (__eo_to_smt t) = SmtType.Bool
 
+structure RuleResultFacts (M : SmtModel) (P : Term) : Prop where
+  true_in_model : eo_interprets M P true
+  has_smt_translation : eo_has_smt_translation P
+
 theorem eo_has_smt_translation_true :
   eo_has_smt_translation (Term.Boolean true) := by
   simp [eo_has_smt_translation, __eo_to_smt, __smtx_typeof]
