CpcMini/Rules/Scope.lean
@@ -107,3 +107,20 @@ theorem correct___eo_prog_scope_impl
   (eo_interprets M (__eo_prog_scope x1 (Proof.pf x2)) true) :=
 by
   exact RuleProofs.correct___eo_prog_scope M hM x1 x2
+
+theorem facts___eo_prog_scope_impl
+    (M : SmtModel) (hM : smt_model_well_typed M) (x1 x2 : Term) :
+  (eo_interprets M x1 true -> eo_interprets M x2 true) ->
+  RuleProofs.eo_has_smt_translation x1 ->
+  RuleProofs.eo_has_smt_translation x2 ->
+  __eo_typeof x1 = Term.Bool ->
+  __eo_typeof x2 = Term.Bool ->
+  __eo_prog_scope x1 (Proof.pf x2) ≠ Term.Stuck ->
+  RuleProofs.RuleResultFacts M (__eo_prog_scope x1 (Proof.pf x2)) :=
+by
+  intro hImp hTrans1 hTrans2 hTy1 hTy2 hProg
+  let hBool : RuleProofs.eo_has_bool_type (__eo_prog_scope x1 (Proof.pf x2)) :=
+    typed___eo_prog_scope_impl M x1 x2 hImp hTrans1 hTrans2 hTy1 hTy2 hProg
+  refine ⟨?_, ?_⟩
+  · exact correct___eo_prog_scope_impl M hM x1 x2 hImp hBool
+  · exact RuleProofs.eo_has_smt_translation_of_has_bool_type _ hBool
